tests/lean/run/subst_heq.lean
@@ -2,3 +2,8 @@ example (a b : nat) (h : a == b) : a + 1 = b + 1 :=
 begin
   subst h
 end
+
+example (a b : nat) (h : a == b) : a + 1 = b + 1 :=
+begin
+  subst_vars
+end
